MathematicalLogic/Notation.lean
@@ -1,37 +1,41 @@
 import Mathlib.Order.BoundedOrder
 import Mathlib.Data.Vector
 
-universe u
+universe u v
 
 notation "[]ᵥ" => Vector.nil
 infixr:67 "∷ᵥ" => Vector.cons
 
-@[notation_class] class NotSymbol (α : Type u) where
-  not : α → α
-
-@[notation_class] class AndSymbol (α : Type u) where
-  and : α → α → α
-
-@[notation_class] class OrSymbol (α : Type u) where
-  or : α → α → α
-
-@[notation_class] class ImpSymbol (α : Type u) where
+class FormulaSymbol (α : Type u) where
+  false : α
   imp : α → α → α
 
-@[notation_class] class IffSymbol (α : Type u) where
-  iff : α → α → α
+namespace FormulaSymbol
 
-@[notation_class] class ForallSymbol (α : Type u) where
-  all : α → α
+variable [FormulaSymbol α] (p q : α)
 
-@[notation_class] class ExistsSymbol (α : Type u) where
-  exist : α → α
+instance : Bot α := ⟨false⟩
 
-prefix:58 "~ " => NotSymbol.not
-infix:56 " ⋁ " => OrSymbol.or
-infix:57 " ⋀ " => AndSymbol.and
-infixr:55 " ⟶ " => ImpSymbol.imp
-infix:55 " ⟷ " => IffSymbol.iff
-prefix:59 "∀' " => ForallSymbol.all
-prefix:59 "∃' " => ExistsSymbol.exist
-attribute [match_pattern] NotSymbol.not OrSymbol.or AndSymbol.and ImpSymbol.imp IffSymbol.iff ForallSymbol.all ExistsSymbol.exist
+infixr:55 " ⟶ " => imp
+attribute [match_pattern] imp
+
+def neg := p ⟶ ⊥
+prefix:58 "~ " => neg
+
+instance : Top α := ⟨~ ⊥⟩
+
+def or := ~ p ⟶ q
+infix:56 " ⋁ " => or
+
+def and := ~ (p ⟶ ~ q)
+infix:57 " ⋀ " => and
+
+def iff := (p ⟶ q) ⋀ (q ⟶ p)
+infix:55 " ⟷ " => iff
+
+end FormulaSymbol
+
+@[notation_class] class EquivSymbol (α : Type u) (β : outParam (Type v)) where
+  equiv : α → α → β
+
+infix:70 " ≈ " => EquivSymbol.equiv
